cleaning

Mergesort.fst
@@ -4,8 +4,6 @@ open FStar.Mul
 open FStar.Math.Lib
 open FStar.IO
 
-// #set-options "--initial_fuel 10 --initial_ifuel 10"
-
 let rec length l : nat =
     match l with
     | [] -> 0
@@ -15,6 +13,10 @@ let rec sorted (l : list int) =
     match l with
     | [] | [ _ ] -> true
     | a :: b :: tl -> a <= b && sorted (b :: tl)
+
+
+// MERGE
+
 
 let rec merge (a : list int) (b : list int)
     : c : list int { length c = length a + length b } =
@@ -26,46 +28,18 @@ let rec merge (a : list int) (b : list int)
         else
             h2 :: merge a t2
 
-(*
 
-let rec take #a (l : list a) (n : nat { n <= length l }) : r : list a { length r = n } =
-    if n = 0 then []
-    else match l with | hd :: tl -> hd :: take tl (n - 1)
+let rec mergedCorrectly (l : list int) (r : list int)
+    : Lemma (sorted l /\ sorted r ==> sorted (merge l r)) =
+    match l, r with
+    | [], _ | _, [] -> ()
+    | h1 :: t1, h2 :: t2 ->
+        mergedCorrectly t1 (h2 :: t2);
+        mergedCorrectly (h1 :: t1) t2
 
-let rec drop #a (l : list a) (n : nat { n <= length l }) : r : list a { length r = length l - n } =
-    if n = 0 then l
-    else match l with | _ :: tl -> drop tl (n - 1)
 
-let rec halve (n : nat { n > 0 }) : d : nat { d < n } =
-    match n with
-    | 0 | 1 -> 0
-    | other -> 1 + halve (n - 2)
- 
-let rec divBy2IsLess (n : nat)
-    : Lemma (halve n <= n) =
-    match n with
-    | 0 | 1 -> ()
-    | other ->
-        divBy2IsLess (other - 1)
+// SPLIT
 
-let nMinusItsHalfIsLess (n : nat) : Lemma (n - halve n <= n) = ()
-*)
-(*
-let split #a (l : list a)
-    : x : (list a & list a) { length (fst x) + length (snd x) = length l } =
-    let len = length l in
-        (take l (halve len), drop l (len - halve len))
-*)
-
-(*
-let rec split #a (s left right : list a)
-    : x : (list a & list b) {  } =
-    match s with
-    | [] -> left, right
-    | h1 :: [] -> h1 :: left, right
-    | h1 :: h2 :: [] -> h1 :: left, h2 :: right
-    | h1 :: h2 :: tl -> split tl (h1 :: left) (h2 :: right)
-*)
 
 let rec split #a (s : list a) : x : (list a & list a) { length (fst x) + length (snd x) = length s } =
     match s with
@@ -77,13 +51,13 @@ let rec split #a (s : list a) : x : (list a & list a) { length (fst x) + length 
         h1 :: l, h2 :: r
 
 let splitLemma #a (s : list a)
-    : Lemma (requires length s > 2)
+    : Lemma (requires length s >= 2)
             (ensures length (fst (split s)) < length s /\ length (snd (split s)) < length s)
     = ()
 
-// let nMinusHalfPlusHalf (n : nat) : Lemma (halve n + (n - halve n) = n) = ()
 
-// #set-options "--initial_fuel 10 --initial_ifuel 10"
+// MERGE SORT
+
 
 let rec mergeSort (l : list int) : Tot (r : list int { length r = length l }) (decreases (length l)) =
     match l with
@@ -93,42 +67,8 @@ let rec mergeSort (l : list int) : Tot (r : list int { length r = length l }) (d
         if a < b then [ a; b ]
         else [ b; a ]
     | other ->
-        // let len = length other in
-        // let left = take other (halve len) in
-        // let right = drop other (len - halve len) in 
-        // merge (mergeSort left) (mergeSort right)
         let (left, right) = split other in
         merge (mergeSort left) (mergeSort right)
-
-
-(*
-let rec sortedCorrectly (l : list int)
-    : Lemma (ensures (sorted (mergeSort l))) (decreases (length l)) =
-    match l with
-    | [] | [ _ ] | [ _; _ ] -> ()
-    | other ->
-        let (left, right) = split other in
-        // assert (sorted (mergeSort left));
-        // assert (sorted (mergeSort right));
-        sortedCorrectly (merge (mergeSort left) (mergeSort right))
-*)
-
-// #reset-options
-
-
-
-// let sorts1 = assert(sorted (mergeSort [ 1; 2; 3 ]))
-// let sorts2 = assert(sorted (mergeSort [ 4; 5; 1 ]))
-// let sorts3 = assert(sorted (mergeSort [ 5; -1 ]))
-// let sorts4 = assert(sorted (mergeSort [ 0; 9; 1; 4; 5 ]))
-
-let rec mergedCorrectly (l : list int) (r : list int)
-    : Lemma (sorted l /\ sorted r ==> sorted (merge l r)) =
-    match l, r with
-    | [], _ | _, [] -> ()
-    | h1 :: t1, h2 :: t2 ->
-        mergedCorrectly t1 (h2 :: t2);
-        mergedCorrectly (h1 :: t1) t2
 
 
 let rec sortReturnsSorted (l : list int)
@@ -137,7 +77,7 @@ let rec sortReturnsSorted (l : list int)
     | [] | [ _ ] | [ _; _ ] -> ()
     | other ->
         let (left, right) = split other in
-        // assert(length left < length other /\ length right < length other); 
+        assert(length left < length other /\ length right < length other); 
         sortReturnsSorted (mergeSort left);
         sortReturnsSorted (mergeSort right);
         mergedCorrectly (mergeSort left) (mergeSort right);
